theories/prob_eff_lang/probblaze/sem_row.v
@@ -19,22 +19,23 @@ Global Instance sem_row_bottom {Σ} : Bottom (sem_row Σ) := sem_row_nil.
 (* TODO: update to use iLblThy s.t. we can use BREL *)
 (* Cons Row *)
 Program Definition sem_row_cons {Σ} (op1 op2 : label) : sem_sig Σ -d> sem_row Σ -d> sem_row Σ :=
-    λ σ ρ, (@SemRow Σ (@LblSig Σ ((([op1], [op2]), σ) :: (sem_row_car ρ))) _ _ ) .
+    λ σ ρ, (@SemRow Σ ((([op1], [op2]), σ) :: (sem_row_car ρ)) _ _ ) .
               (* (λ e1 e2, λne Φ, ∃ (op' : label) (v1 v2 : val), 
                               ⌜ e1 = (do: op' v1)%E ⌝ ∗ ⌜ e2 = (do: op' v2)%E ⌝ ∗
                                if decide (op = op') then 
                                  ▷ ((pmono_prot_car σ) v1 v2 Φ)
                                else
                                  (pmono_prot_car (sem_row_car ρ)) (do: op' v1)%E (do: op' v2)%E Φ)%I) _). *)
-Next Obligation. intros ?????. iIntros (????) "#H1 H2". iApply to_iThy_cons. iDestruct (to_iThy_cons with "H2") as "H2".
-                 iDestruct "H2" as "[(%&%&%&%&%&->&%&->&%&Hσ&#Hcont)|(%&%&%&%&%&%&%&%&%&->&%&->&%&Hσ&#Hcont)]"; [iLeft|iRight].
-                 - iExists _,_,_,_,_. do 4 (iSplit; [iPureIntro;done|]). iFrame.
-                   iModIntro. iIntros (??) "HS". iDestruct ("Hcont" with "HS") as "HΦ".
-                   by iApply "H1".
-                 - simpl. iExists _,_,_. iFrame. iSplit; [iPureIntro; done|].
-                   iExists _,_. do 4 (iSplit;[iPureIntro;done|]).
-                   iIntros "!# % % HS". iDestruct ("Hcont" with "HS") as "HΦ".
-                   by iApply "H1".
+Next Obligation.
+  intros ?????. iIntros (????) "#H1 H2". iApply to_iThy_cons. iDestruct (to_iThy_cons with "H2") as "H2".
+  iDestruct "H2" as "[(%&%&%&%&%&->&%&->&%&Hσ&#Hcont)|(%&%&%&%&%&%&%&%&%&->&%&->&%&Hσ&#Hcont)]"; [iLeft|iRight].
+  - iExists _,_,_,_,_. do 4 (iSplit; [iPureIntro;done|]). iFrame.
+    iModIntro. iIntros (??) "HS". iDestruct ("Hcont" with "HS") as "HΦ".
+    by iApply "H1".
+  - simpl. iExists _,_,_. iFrame. iSplit; [iPureIntro; done|].
+    iExists _,_. do 4 (iSplit;[iPureIntro;done|]).
+    iIntros "!# % % HS". iDestruct ("Hcont" with "HS") as "HΦ".
+    by iApply "H1".
 Qed.
 Next Obligation.
   iIntros (????????) "H". 
@@ -43,7 +44,10 @@ Next Obligation.
   - destruct σ. iDestruct sem_sig_prop as "H1". iExists _, _.
     iDestruct ("H1" with "Hσ") as (????) "H". iExists op0, op3, v1,v2.
     iDestruct "H" as "(-> & ->)". done.
-  - Admitted.
+  - apply in_iLblSig in H as (X' & ->).
+    iDestruct (sem_sig_prop with "Hσ") as (op3 op4 v1 v2) "(-> & ->)".
+    iExists _,_,_,_,_,_. done.
+Qed.
 
 (* Recursive Row *)
 Definition sem_row_rec {Σ} (R : sem_row Σ → sem_row Σ) `{Contractive R} : sem_row Σ :=
@@ -58,12 +62,22 @@ Proof. rewrite /sem_row_rec {1} fixpoint_unfold //. Qed.
    Proof. f_equiv. apply non_dep_fun_equiv.  apply non_dep_fun_equiv. rewrite {1}sem_row_rec_unfold //. Qed. *)
 
 (* Flip-Bang Row *)
-(* TOOD: Find a better way to make iLblSig a subtype of iLblThy -- the properties of the elements in the list are not preserved *)                          
+(* This is essentially to_iThyIfMono *)
 Definition iThyIfMono_iLblSig {Σ} (m: mode) (L : iLblSig Σ) : iLblSig Σ :=
-  @LblSig Σ (map (λ '(l1s, l2s, X), (l1s, l2s, sem_sig_flip_mbang m X)) L).
+  (map (λ '(l1s, l2s, X), (l1s, l2s, sem_sig_flip_mbang m X)) L).
 
+(* TODO: does this hold? What if I forget the sem_sig structure? *)
+(* Lemma iThyIfMono_iLblSigMS {Σ} (L : iLblSig Σ) : 
+     iThyIfMono_iLblSig MS L = L.
+   Proof.
+     (* induction L as [|((?,?),?)]; [done|rewrite //= IHL].
+        unfold sem_sig_flip_mbang. simpl. done.
+          destruct L.
+        by induction L as [|((?,?),?)]; [|rewrite //= IHL]. Q. *)
+   Admitted.  *)
+  
 Program Definition sem_row_flip_mbang {Σ} (m : mode) (ρ : sem_row Σ) : sem_row Σ := 
-  @SemRow Σ (@LblSig Σ (iThyIfMono_iLblSig m ρ)) _ _.
+  @SemRow Σ (iThyIfMono_iLblSig m ρ) _ _.
 Next Obligation.
   iIntros (???????) "#HΦ Hσ". 
   iDestruct "Hσ" as (????????? -> ? -> ?) "(HX & #Hcont)".
@@ -72,14 +86,15 @@ Next Obligation.
   iIntros (??) "!# HS". iApply "HΦ". by iApply "Hcont".
 Qed.
 Next Obligation.
-  iIntros (??????) "Hρ". destruct m.
-  - simpl. iDestruct "Hρ" as (????????? -> ? -> ?) "(HX & #Hcont)". simpl in *. admit.
-  - simpl.
-Admitted.
-
+  iIntros (??????) "Hρ".
+  simpl. iDestruct "Hρ" as (????????? -> ? -> ?) "(HX & #Hcont)".
+  apply in_iLblSig in H as (X' & ->).
+  iDestruct (sem_sig_prop with "HX") as (op3 op4 v1 v2) "(-> & ->)".
+  iExists _,_,_,_,_,_. done.
+Qed.
 (* Notations. *)
 Notation "⟨⟩" := (sem_row_nil) : sem_row_scope.
-Notation "opσ · ρ" := (sem_row_cons opσ.1%S opσ.2%S ρ%R) (at level 80, right associativity) : sem_row_scope.
+Notation "opσ · ρ" := (sem_row_cons opσ.1.1 opσ.1.2 opσ.2 ρ) (at level 80, right associativity) : sem_row_scope.
 Notation "¡[ m ] ρ" := (sem_row_flip_mbang m ρ) (at level 10) : sem_row_scope.
 Notation "¡ ρ" := (sem_row_flip_mbang OS ρ) (at level 10) : sem_row_scope.
 Notation "'μᵣ' θ , ρ " := (sem_row_rec (λ θ, ρ%R)) (at level 50) : sem_row_scope.
@@ -126,12 +141,58 @@ Section once_row.
     row_le_mfbang_elim : (⊢ (¡ ρ%R) ≤ᵣ ρ%R)
   }.
 
-  (* TODO: figure out typeclasses to use OnceR *)
-  Global Instance monoprot_once `{probblazeRGS Σ} (ρ : sem_row Σ) `{! OnceR ρ } : MonoProt (to_iThy ρ).
+  Lemma iLblSig_car_thing {Σ} (ρ : iLblSig Σ) :
+   ∃ ρ' : iLblThy Σ, iLblSig_to_iLblThy ρ = ρ'
   Proof.
-    constructor. iIntros (????) "HP Hρ".
-    inv OnceR0. (* iApply row_le_mfbang_elim0. *)
-  Admitted. 
+    simpl. done.
+  Qed. 
+    
+  (* TODO: This should be provable, but the records and coercions are annoying*)
+  Lemma iThyIfMono_iLblSig_to_iThyIfMono {Σ} (m : mode) (ρ : sem_row Σ) :
+    iLblSig_to_iLblThy (sem_row_flip_mbang m ρ) = to_iThyIfMono m (iLblSig_to_iLblThy ρ).
+  Proof.
+    unfold iLblSig_to_iLblThy.
+    (* case m; last first.
+       { rewrite to_iThyIfMonoMS. unfold sem_row_flip_mbang. destruct ρ. simpl. rewrite (iThyIfMono_iLblSigMS ρ). *)
+    destruct ρ as [l Hmono Hprop].
+    induction l; first done. intros.
+    simpl. destruct a as [[l1s l2s] σ]. rewrite IHl; last done.
+    - iIntros (????) "#HΦ HlΨ".
+      iPoseProof Hmono as "Hmcons".
+      iDestruct "HlΨ" as (l1s' l2s' X) "(%Hin & HXΦ)".
+      (* iExists _,_,_. iSplit; first done. *)
+      iDestruct ("Hmcons" with "HΦ") as "HΨ".
+      iAssert (to_iThy (iLblSig_to_iLblThy ((l1s,l2s,σ) :: l)) v1 v2 Φ) with "[HXΦ]" as "Htemp".
+      { iExists _,_,_. iSplit; [iPureIntro; by apply elem_of_list_further|]. done. }
+      iDestruct ("HΨ" with "Htemp") as "HΦ'".
+      iDestruct "HΦ'" as (l1s'' l2s'' X') "H".
+      iExists _,_,_.
+  Admitted.         
+
+  Definition mono_prot_on_prop {Σ} (Ψ : sem_row Σ) (P : iProp Σ) : iProp Σ :=
+    □ (∀ e1 e2 Φ, (to_iThy (iLblSig_to_iLblThy Ψ)) e1 e2 Φ -∗ P -∗ (to_iThy (iLblSig_to_iLblThy Ψ)) e1 e2 (λ w1 w2, Φ w1 w2 ∗ P))%I.
+
+  Lemma mono_prot_on_prop_monotonic {Σ} (σ : sem_row Σ) : 
+    (⊢ ∀ P, mono_prot_on_prop σ P) ↔ MonoProt (to_iThy (iLblSig_to_iLblThy σ)).
+  Proof.
+    split.
+    - iIntros (H). constructor. iIntros (v1 v2 Φ Φ') "Hpost HΨ".
+      iDestruct (H with "HΨ Hpost") as "H".
+      iApply (sem_row_mono _ σ with "[] H").
+      iIntros "!# % % [HΦ HPost]". by iApply "HPost".
+    - iIntros (H) "%P %v1 %v2 %Φ !# Hσ HP". inv H.
+      iApply (monotonic_prot with "[HP] Hσ"). iIntros (??) "$ //".
+  Qed.
+
+  Global Instance monoprot_once `{probblazeRGS Σ} (ρ : sem_row Σ) `{! OnceR ρ } : MonoProt (to_iThy (iLblSig_to_iLblThy ρ)).
+  Proof.
+    apply mono_prot_on_prop_monotonic. iIntros (????) "!# HΨ HP".
+    inv OnceR0. iDestruct row_le_mfbang_elim0 as "(H1 & H2)".
+    iApply "H1".
+    rewrite (iThyIfMono_iLblSig_to_iThyIfMono OS).
+    iApply iThy_le_to_iThy_to_iThyIfMono.
+    iFrame. iIntros "!> %% $".
+  Qed.
 End once_row.
 
 Section row_sub_typing.
@@ -153,23 +214,39 @@ Section row_sub_typing.
   Proof. iApply to_iThy_le_bot. Qed.
 
   (* TODO: figure out how to extend sem_rows *)
-  (* Lemma row_le_cons_comp (ρ ρ' : sem_row Σ) (op op' : label) (σ σ' : sem_sig Σ) : 
-       σ ≤ₛ σ' -∗ ρ ≤ᵣ ρ' -∗ 
-       [([op], [op'], σ)] ⋅ ρ ≤ᵣ ([op], [op'], σ') · ρ'.
-     Proof.
-       iIntros "#Hσσ' #Hρρ'". rewrite /sem_row_cons /=. 
-       iIntros (???) "!# (%op' & %v1' & %v2' & -> & -> & H)".
+  Lemma row_le_cons_comp (ρ ρ' : sem_row Σ) (op op' : label) (σ σ' : sem_sig Σ) : 
+    σ ≤ₛ σ' -∗ ρ ≤ᵣ ρ' -∗ sem_row_cons op op' σ ρ ≤ᵣ sem_row_cons op op' σ' ρ'.
+    (* (((op, op'), σ) ⋅ ρ) ≤ᵣ ((op, op'), σ') · ρ'. *)
+  Proof.
+    iIntros "#Hσσ' #Hρρ'". (* rewrite /sem_row_cons /=. *)
+    unfold row_le. simpl.
+    iSplit.
+    - admit.
+    - iDestruct "Hρρ'" as "(_&#(#Hvalid & #Hdistinct))".
+      iSplit.
+      + iModIntro. iIntros "#H".
+        iDestruct (valid_submseteq with "H") as "Hρ'".
+        { instantiate (1 := iLblSig_to_iLblThy ρ').
+          apply submseteq_cons. set_solver. }
+        iDestruct ("Hvalid" with "Hρ'") as "Hρ".
+        iSplit.
+        * iDestruct "H" as "(H1 & H2)". unfold valid_l.
+          admit.
+        * admit.
+      + admit.
+    (* iIntros (???) "!# (% & % & % & % & % & % & -> & -> & H)".
        iExists op', v1', v2'; do 2 (iSplit; first done).
        destruct (decide (op = op')); first (by iApply "Hσσ'"). 
-       by iApply "Hρρ'".
-     Qed.
-     
-     Lemma row_le_swap_second {Σ} (op op' : label) (σ σ' : sem_sig Σ) (ρ : sem_row Σ) : 
-       op ≠ op' →
-       ⊢ (op, σ) · (op', σ') · ρ ≤ᵣ (op', σ') · (op, σ) · ρ. 
-     Proof. 
-       iIntros (Hneq). rewrite /sem_row_cons /=.
-       iIntros (???) "!# (%op'' & %v1'' & %v2'' & %Heq1 & %Heq2 & H)". simpl.
+       by iApply "Hρρ'". *)
+  Admitted. 
+  
+  Lemma row_le_swap_second `{probblazeRGS Σ} (op1 op1' op2 op2' : label) (σ σ' : sem_sig Σ) (ρ : sem_row Σ) : 
+    op1 ≠ op1' →
+    op2 ≠ op2' →
+    ⊢ (op1, op2, σ) · (op1', op2', σ') · ρ ≤ᵣ (op1', op2', σ') · (op1, op1', σ) · ρ. 
+  Proof. 
+    iIntros (Hneq). rewrite /sem_row_cons /=.
+    (* iIntros (???) "!# (%op'' & %v1'' & %v2'' & %Heq1 & %Heq2 & H)". simpl.
        destruct (decide (op = op'')) as [->|].
        - iExists op'', v1'', v2''. do 2 (iSplit; first done).
          rewrite decide_False; last done.
@@ -183,18 +260,21 @@ Section row_sub_typing.
            simplify_eq. rewrite decide_False //.
            iExists op''', v1''', v2'''. do 2 (iSplit; first done).
            rewrite decide_False //.
-     Qed.
-     
-     Corollary row_le_swap_third {Σ} (op op' op'' : label) (σ σ' σ'' : sem_sig Σ) (ρ : sem_row Σ) : 
-       op ≠ op' → op' ≠ op'' → op'' ≠ op →
-       ⊢ (op, σ) · (op', σ') · (op'', σ'') · ρ ≤ᵣ (op'', σ'') · (op, σ) · (op', σ') · ρ. 
-     Proof. 
-       iIntros (???). 
+     Qed. *)
+  Admitted. 
+  
+  Corollary row_le_swap_third `{probblazeRGS Σ} (op1 op1' op1'' op2 op2' op2'' : label) (σ σ' σ'' : sem_sig Σ) (ρ : sem_row Σ) : 
+    op1 ≠ op1' → op1' ≠ op1'' → op1'' ≠ op1 →
+    op2 ≠ op2' → op2' ≠ op2'' → op2'' ≠ op2 →
+    ⊢ (op1, op2,  σ) · (op1', op2', σ') · (op1'', op2'', σ'') · ρ ≤ᵣ (op1'', op2'', σ'') · (op1, op2, σ) · (op1', op2', σ') · ρ. 
+  Proof. 
+    (* iIntros (??????). 
        iApply row_le_trans; first iApply row_le_cons_comp; [iApply sig_le_refl|by iApply row_le_swap_second|].
        by iApply row_le_swap_second.
-     Qed.
-     
-     Corollary row_le_swap_fourth {Σ} (op op' op'' op''' : label) (σ σ' σ'' σ''': sem_sig Σ) (ρ : sem_row Σ) : 
+     Qed. *)
+  Admitted.
+  
+  (* Corollary row_le_swap_fourth {Σ} (op op' op'' op''' : label) (σ σ' σ'' σ''': sem_sig Σ) (ρ : sem_row Σ) : 
        op ≠ op' → op ≠ op'' → op ≠ op''' → op' ≠ op'' → op' ≠ op''' → op'' ≠ op''' → 
        ⊢ (op, σ) · (op', σ') · (op'', σ'') · (op''', σ''') · ρ ≤ᵣ 
          (op''', σ''') · (op, σ) · (op', σ') · (op'', σ'') · ρ.
@@ -212,72 +292,118 @@ Section row_sub_typing.
     ⊢ R (μᵣ θ, R θ) ≤ᵣ (μᵣ θ, R θ).
   Proof. rewrite - {1} sem_row_rec_unfold. iApply row_le_refl. Qed.
 
-  (* TODO: typeclasses... *)
   Lemma row_le_mfbang_intro (m : mode) (ρ : sem_row Σ) :
     ⊢ ρ ≤ᵣ ¡[ m ] ρ. 
-  Proof. 
-  (*   rewrite /sem_row_flip_mbang. iIntros (???) "!# Hρ". simpl.
-       destruct m; [|done]. simpl.
-       iExists Q. iFrame. iModIntro.
-       iIntros "% % $ //".
-     Qed. *)
-  Admitted. 
-    
+  Proof.
+    rewrite /sem_row_flip_mbang. unfold row_le. simpl.
+    iSplit.
+    - iIntros (???) "!#". case m; last first.
+      { rewrite iThyIfMono_iLblSig_to_iThyIfMono. rewrite to_iThyIfMonoMS. iIntros "$". }
+      rewrite iThyIfMono_iLblSig_to_iThyIfMono.
+      iIntros "(%&%&%&%Hin&Ht)". iExists _,_, (iThyMono X).
+      iSplit.
+      { iPureIntro. induction (iLblSig_to_iLblThy ρ); first by apply elem_of_nil in Hin.
+        simpl. destruct a as [[l1s' l2s'] X']. apply elem_of_cons in Hin as [Hin| Hin].
+        - simplify_eq. apply elem_of_list_here.
+        - apply IHi in Hin. by apply elem_of_list_further. }
+      iDestruct "Ht" as (?????->?->?) "(HX & #Hcont)".
+      iExists _,_,_,_,_. repeat (iSplit; first done).
+      iSplitL; last iFrame "#".
+      iExists S. iSplitL; first iFrame.
+      iIntros (??) "!> $".
+    - iSplit.
+      + iIntros "!# H". iApply valid_to_iThyIfMono. by rewrite -iThyIfMono_iLblSig_to_iThyIfMono.
+      + iIntros "!# %Hd". iPureIntro. erewrite distinct_to_iThyIfMono. by rewrite -iThyIfMono_iLblSig_to_iThyIfMono.
+  Qed.
+
   Lemma row_le_mfbang_elim_ms (ρ : sem_row Σ) :
     ⊢ ¡[MS] ρ ≤ᵣ ρ. 
   Proof. 
-    (* rewrite /sem_sig_flip_mbang. 
-       iIntros (v1 v2 Φ) "!# H". done. 
-     Qed. *)
-  Admitted. 
-
-  (* Lemma to_iThy_le_iThyIfMono_iLblSig (L M : iLblSig Σ) :
-       L ≤ᵣ M -∗ (iThyIfMono_iLblSig L) ≤ᵣ (iThyIfMono_iLblSig M). *)
-  (* TODO: proof a theorem like iThy_le_iThyMono for iThyIfMono_iLblSig *)
+    rewrite /sem_row_flip_mbang. unfold row_le. simpl.
+    rewrite iThyIfMono_iLblSig_to_iThyIfMono. rewrite to_iThyIfMonoMS.
+    iApply to_iThy_le_refl.
+  Qed. 
+    
   Lemma row_le_mfbang_comp m m' (ρ ρ' : sem_row Σ) :
     m' ≤ₘ m -∗ ρ ≤ᵣ ρ' -∗
     (¡[m] ρ) ≤ᵣ (¡[m'] ρ').
   Proof. 
-  (*   iIntros "#Hlem #Hleσ". destruct m.
-       - iDestruct (mode_le_OS_inv with "Hlem") as "->".
-         rewrite /row_le /sem_row_flip_mbang /tc_opaque.
-         by iApply iThy_le_iThyMono.
-       - iApply row_le_trans; first iApply row_le_mfbang_elim_ms. 
-         iApply row_le_trans; first iApply (row_le_mfbang_intro m').
-         rewrite /row_le /sem_row_flip_mbang /tc_opaque.
-         by iApply iThy_le_iThyIfMono.
-     Qed. *)
-  Admitted. 
+    iIntros "#Hlem #Hleσ". destruct m.
+    - iDestruct (mode_le_OS_inv with "Hlem") as "->".
+      rewrite /row_le /sem_row_flip_mbang /tc_opaque. 
+      rewrite !iThyIfMono_iLblSig_to_iThyIfMono.
+      iSplit.
+      { iIntros (???) "!# H". iApply iThy_le_to_iThy_to_iThyIfMono.
+        iDestruct (iThy_le_to_iThyIfMono_to_iThy with "H") as "H".
+        iApply (iThy_le_iThyIfMono with "[][$H]").
+        iDestruct "Hleσ" as "($ & _)". }
+      iSplit.
+      + iIntros "!# H". iDestruct (valid_to_iThyIfMono with "H") as "H".
+        iDestruct "Hleσ" as "(_&Hleσ&_)". iDestruct ("Hleσ" with "H") as "H". by iDestruct (valid_to_iThyIfMono with "H") as "$".
+      + iIntros "!# Hd". iDestruct "Hleσ" as "(_&_&Hleσ)". unfold distinct'. repeat rewrite -distinct_to_iThyIfMono. by iApply "Hleσ".
+    - iApply row_le_trans; first iApply row_le_mfbang_elim_ms. 
+      iApply row_le_trans; first iApply (row_le_mfbang_intro m').
+      rewrite /row_le /sem_row_flip_mbang /tc_opaque.
+      rewrite !iThyIfMono_iLblSig_to_iThyIfMono.
+      iSplit.
+      { iIntros (???) "!# H". iApply iThy_le_to_iThy_to_iThyIfMono.
+        iDestruct (iThy_le_to_iThyIfMono_to_iThy with "H") as "H".
+        iApply (iThy_le_iThyIfMono with "[][$H]").
+        iDestruct "Hleσ" as "($ & _)". }
+       iSplit.
+      + iIntros "!# H". iDestruct (valid_to_iThyIfMono with "H") as "H".
+        iDestruct "Hleσ" as "(_&Hleσ&_)". iDestruct ("Hleσ" with "H") as "H". by iDestruct (valid_to_iThyIfMono with "H") as "$".
+      + iIntros "!# Hd". iDestruct "Hleσ" as "(_&_&Hleσ)". unfold distinct'. repeat rewrite -distinct_to_iThyIfMono. by iApply "Hleσ".
+  Qed. 
   
-  (* Lemma row_le_mfbang_dist_cons {Σ} op m σ (ρ : sem_row Σ) :
-       ⊢ ¡[ m ] ((op, σ) · ρ) ≤ᵣ (op, ¡[ m ] σ)%S · (¡[ m ] ρ).
-     Proof. 
-       rewrite /sem_row_flip_mbang. iIntros (???) "!# H". simpl.
+  Lemma row_le_mfbang_dist_cons `{probblazeRGS Σ} op1 op2 m σ (ρ : sem_row Σ) :
+    ⊢ ¡[ m ] ((op1, op2, σ) · ρ) ≤ᵣ (op1, op2, ¡[ m ] σ)%S · (¡[ m ] ρ).
+  Proof. 
+  (*   rewrite /sem_row_flip_mbang. iIntros (???) "!# H". simpl.
        destruct m; simpl; [|done]. 
        iDestruct "H" as (Q') "((%op' & %v1' & %v2' & -> & -> & H) & Hpost)".
        iExists op', v1', v2'. do 2 (iSplit; first done).
        destruct (decide (op = op')); first iNext; iExists Q'; iFrame. 
-     Qed.
-     
-     Global Instance row_cons_once {Σ} (ρ : sem_row Σ) op (σ : sem_sig Σ) `{! OnceS σ, ! OnceR ρ } :
-       OnceR ((op, σ) · ρ)%R.
-     Proof.
-       constructor. inv OnceS0. inv OnceR0.
-       iApply row_le_trans; first iApply row_le_mfbang_dist_cons.
+     Qed. *)
+  Admitted. 
+  
+  Global Instance row_cons_once `{probblazeRGS Σ} (ρ : sem_row Σ) op1 op2 (σ : sem_sig Σ) `{! OnceS σ, ! OnceR ρ } :
+    OnceR ((op1, op2, σ) · ρ)%R.
+  Proof.
+    constructor. inv OnceS0. inv OnceR0.
+    (* iApply row_le_trans; first iApply row_le_mfbang_dist_cons.
        iApply row_le_cons_comp; [iApply sig_le_mfbang_elim|iApply row_le_mfbang_elim0].
      Qed. *)
+  Admitted. 
   
   Lemma row_le_mfbang_idemp m (ρ : sem_row Σ) :
     ⊢ (¡[ m ] (¡[ m ] ρ)) ≤ᵣ ((¡[ m ] ρ)).
-  (* Proof. 
-       iIntros (v1 v2 Φ) "!# H".
-       destruct m; [|done]. simpl.    
-       iDestruct "H" as (Q') "((%Q'' & Hρ & HPost') & HPost)". 
-       iExists Q''. iFrame. 
-       iIntros (??) "!> HQ''".
-       iApply "HPost". by iApply "HPost'".
-     Qed. *)
-  Admitted. 
+  Proof.
+    case m; last apply row_le_mfbang_elim_ms.
+    unfold row_le. simpl.
+    iSplit.
+    - rewrite !iThyIfMono_iLblSig_to_iThyIfMono. 
+      iIntros (???) "!# (%&%&%&%Hin&HX)".
+      iInduction (iLblSig_to_iLblThy ρ) as [|a i] "IH";  first by apply elem_of_nil in Hin.
+      destruct a as [[l1s' l2s'] X']. apply elem_of_cons in Hin as [Hin| Hin].
+      + iExists l1s', l2s', (iThyMono X').
+        iSplit; last first.
+        { simplify_eq. simpl.
+          iDestruct "HX" as (?????->?->?) "((% & (% & (HX' & Hcont)) & H3) & #H1)".
+          iExists _,_,_,_,_. repeat (iSplit; first done).
+          iSplitL; last done.
+          iExists Q'0. iFrame. iIntros (??) "!> HQ'0". iApply "H3". by iApply "Hcont". }
+        iPureIntro.
+        simplify_eq. simpl. apply elem_of_list_here.
+      + iDestruct ("IH" $! Hin) as "IH'".
+        iDestruct ("IH'" with "HX") as "Hi".
+        iDestruct "Hi" as (???) "(%Hin' & HX)".
+        iExists  l1s0, l2s0, X0. iFrame.
+        iPureIntro. set_solver. 
+    - iSplit; iModIntro.
+      + rewrite !iThyIfMono_iLblSig_to_iThyIfMono. rewrite -!valid_to_iThyIfMono. iIntros "$".
+      + rewrite !iThyIfMono_iLblSig_to_iThyIfMono. unfold distinct'. rewrite -!distinct_to_iThyIfMono. iIntros "$".
+  Qed. 
 
   Global Instance row_fbang_once (ρ : sem_row Σ) : OnceR (¡ ρ)%R.
   Proof. constructor. iApply row_le_mfbang_idemp. Qed.
@@ -296,14 +422,13 @@ Section row_sub_typing.
     - iApply row_le_refl.
   Qed.
 
-  (* TODO: finish this proofs *)
+ 
   Lemma row_le_mfbang_elim_nil m :
      ⊢ ¡[m] ⟨⟩%R ≤ᵣ (⟨⟩%R : sem_row Σ).
   Proof. 
     destruct m; simpl; last iApply row_le_mfbang_elim_ms.
-    (* iIntros (???) "!# (% & [] & _)".
-     Qed. *)
-  Admitted.
+    iApply to_iThy_le_bot.
+  Qed.
   
   Global Instance row_nil_once : OnceR (⟨⟩ : sem_row Σ)%R.
   Proof. constructor. iApply row_le_mfbang_elim_nil. Qed.
@@ -312,11 +437,8 @@ Section row_sub_typing.
     (∀ θ, ¡[ m ] (R θ) ≤ᵣ (R θ)) -∗ ¡[ m ] (μᵣ θ, R θ) ≤ᵣ (μᵣ θ, R θ).
   Proof. 
     iIntros "Hle". destruct m; last iApply row_le_mfbang_elim_ms.
-    (* iIntros (???) "!# (%Φ' & H & HP)". simpl.
-       iApply sem_row_rec_unfold_iThy. rewrite sem_row_rec_unfold_iThy.
-       iApply "Hle". iExists Φ'. simpl. iFrame.
-     Qed. *)
-  Admitted.
+    rewrite sem_row_rec_unfold. iApply "Hle".
+  Qed.
   
   Global Instance row_rec_once (R : sem_row Σ → sem_row Σ) `{Contractive R} :
     (∀ θ, OnceR (R θ)) → OnceR (μᵣ θ, R θ)%R.
@@ -331,26 +453,11 @@ End row_sub_typing.
 Section row_type_sub.
 
   (* Substructurality relation on rows wrt to types and environments *)
-  
-  Definition mono_prot_on_prop {Σ} (Ψ : sem_row Σ) (P : iProp Σ) : iProp Σ :=
-    □ (∀ e1 e2 Φ, (to_iThy Ψ) e1 e2 Φ -∗ P -∗ (to_iThy Ψ) e1 e2 (λ w1 w2, Φ w1 w2 ∗ P))%I.
-
-  (* Lemma mono_prot_on_prop_monotonic {Σ} (σ : sem_sig Σ) : 
-       (⊢ ∀ P, mono_prot_on_prop σ P) ↔ MonoProt σ.
-     Proof.
-       split.
-       - iIntros (H). constructor. iIntros (v1 v2 Φ Φ') "Hpost HΨ".
-         iDestruct (H with "HΨ Hpost") as "H".
-         iApply (pmono_prot_prop _ σ with "[] H").
-         { iIntros "!# % % [HΦ HPost]". by iApply "HPost". }
-       - iIntros (H) "%P %v1 %v2 %Φ !# Hσ HP". inv H.
-         iApply (monotonic_prot with "[HP] Hσ"). iIntros (??) "$ //".
-     Qed. *)
-  
+    
   Class RowTypeSub {Σ} (ρ : sem_row Σ) (τ : sem_ty Σ) := {
     row_type_sub : ⊢ (∀ v1 v2, mono_prot_on_prop ρ (τ v1 v2))
   }.
-
+ 
   Global Instance row_type_sub_once `{probblazeRGS Σ} (ρ : sem_row Σ) (τ : sem_ty Σ) `{! OnceR ρ} : RowTypeSub ρ τ.
   Proof.
     constructor.
@@ -360,23 +467,22 @@ Section row_type_sub.
   Qed.
   
 End row_type_sub.
-(* TODO: finish once env is defined *)
-(* Section row_env_sub.
-   
-     Class RowEnvSub {Σ} (ρ : sem_row Σ) (Γ : env Σ) := {
-       row_env_sub : ⊢ (∀ γ, mono_prot_on_prop ρ (Γ ⊨ₑ γ))
-     }.
-     
-     Global Instance row_env_sub_once {Σ} (ρ : sem_row Σ) (Γ : env Σ) `{! OnceR ρ} : RowEnvSub ρ Γ.
-     Proof.
-       constructor.
-       iIntros (γ v Φ) "!# Hρ HΓ".
-       iApply (monotonic_prot v Φ (λ w', Φ w' ∗ Γ ⊨ₑ γ)%I with "[HΓ] Hρ").
-       iIntros "% $ //".
-     Qed.
-     
-   End row_env_sub. *)
+Section row_env_sub.
+
+  Class RowEnvSub {Σ} (ρ : sem_row Σ) (Γ : env Σ) := {
+    row_env_sub : ⊢ (∀ γ, mono_prot_on_prop ρ (Γ ⊨ₑ γ))
+  }.
+  
+  Global Instance row_env_sub_once `{probblazeRGS Σ} (ρ : sem_row Σ) (Γ : env Σ) `{! OnceR ρ} : RowEnvSub ρ Γ.
+  Proof.
+    constructor.
+    iIntros (γ v1 v2 Φ) "!# Hρ HΓ".
+    iApply (monotonic_prot v1 v2 Φ (λ w1' w2', Φ w1' w2' ∗ Γ ⊨ₑ γ)%I with "[HΓ] Hρ").
+    iIntros "% % $ //".
+  Qed.
+  
+End row_env_sub.
 
 (* Notations *)
-(* Notation "ρ ᵣ⪯ₑ Γ" := (RowEnvSub ρ%R Γ%T) (at level 80). *)
+Notation "ρ ᵣ⪯ₑ Γ" := (RowEnvSub ρ%R Γ%T) (at level 80).
 Notation "ρ ᵣ⪯ₜ τ" := (RowTypeSub ρ%R τ%T)%I (at level 80).
